ClickMG.v
@@ -39,8 +39,23 @@ Section TokenMG.
   (* L.ack -> L.req *)
   (* CLK- -> L.req *)
   (* R.req -> L.req *)
+  (* ENVIRONMENT constraint: we expect handshakes to obey a 2-phase handshake
+     protocol, so we don't expect an input on left_req until left_ack has been
+     updated by the controller. *)
   | left_ack_left_req : stage_place left_ack left_req
+  (* TIMING constraint: changes inside the controller propogate faster than
+     communication between controllers. In the controller, if this is not
+     respected, it will lead to an error state as the clock component will not
+     be stable when the new inputs arrive. *)
+  (* NOTE: really, this should perhaps be that CLK- must occur before BOTH
+     left_req and right_ack inputs change, not just either one... Since this
+     can't be encoded simply as a marked graph, perhaps it needs to be encoded
+     into the environment of latch_stage? *)
   | clk_fall_left_req : stage_place clk_fall left_req
+  (* TIMING constraint: changes inside the controller propogate faster than
+     communication between controllers. In other words, wait for state0 to be
+     propogated to both left_ack AND right_req before accepting input on
+     left_req. *)
   | right_req_left_req : stage_place right_req left_req
 
   (* CLK+ -> L.ack *)
@@ -50,13 +65,17 @@ Section TokenMG.
   | clk_rise_right_req : stage_place clk_rise right_req
 
   (* R.req -> R.ack *)
+  (* ENVIRONMENT constraint: we expect handshakes to obey a 2-phase handshake
+     protocol, so we don't expect an input on right_ack until right_req has been
+     updated by the controller  *)
   | right_req_right_ack : stage_place right_req right_req
   
   (* CLK- -> R.ack *)
   (* L.ack -> R.ack *)
+  (* TIMING constraint: See the note on clk_fall_left_req. *)
   | clk_fall_right_ack : stage_place clk_fall right_ack
+  (* TIMING constraint: See the note on right_req_left_req. *)
   | left_ack_right_ack : stage_place left_ack right_ack
-  
 
   (* CLK+ -> CLK- *)
   | clock_fall : stage_place clk_rise clk_fall
@@ -246,20 +265,11 @@ Section SS_to_TokenMG.
 
 
 
-  Notation "σ1 'R{' t '}' σ2" := (relate_trace name (latch_stage l) (stage_MG_SS l in_flag)
-                      (σR l) init_stage_MG_state
-                      σ1 t σ2)
-    (left associativity, at level 92).
-
-
-  Definition latch_clk_component := clk_component (latch_input l) (latch_output l)
-                                      ctrl_reset_n (latch_clk l) (latch_state0 l)
-                                      (latch_to_token_flag l).
   
 
   Lemma left_req_inversion : forall σ σ' v,
     latch_stage l ⊢ σ →{Some (Event (req (latch_input l)) v)} Some σ' ->
-    stable latch_clk_component σ 
+    stable (latch_clk_component l) σ 
     /\ v = neg_value (σ (req (latch_input l))).
   Proof.
     intros.
@@ -272,13 +282,11 @@ Section SS_to_TokenMG.
   Admitted.
   Lemma right_ack_inversion : forall σ σ' v,
     latch_stage l ⊢ σ →{Some (Event (ack (latch_output l)) v)} Some σ' ->
-    stable latch_clk_component σ.
+    stable (latch_clk_component l) σ.
   Admitted.
-  Definition latch_left_ack_component :=
-    ack_i_output (latch_input l) (latch_state0 l) (latch_to_token_flag l).
   Lemma left_ack_inversion : forall σ σ' v,
     latch_stage l ⊢ σ →{Some (Event (ack (latch_input l)) v)} Some σ' ->
-    ~ stable latch_left_ack_component σ.
+    ~ stable (latch_left_ack_component l) σ.
   Admitted.
   Lemma right_req_inversion : forall σ σ' v,
     latch_stage l ⊢ σ →{Some (Event (req (latch_output l)) v)} Some σ' ->
@@ -287,9 +295,247 @@ Section SS_to_TokenMG.
   Lemma clk_inversion : forall σ σ' v,
     latch_stage l ⊢ σ →{Some (Event (latch_clk l) v)} Some σ' ->
        σ (latch_clk l) = σ (latch_old_clk l)
-    /\ ~ stable latch_clk_component σ.
+    /\ ~ stable (latch_clk_component l) σ.
   Admitted.
 
+
+  (** If σ1 R{t} σ2, then the stage_relation_property will hold on σ1 and
+  (state_to_marking σ2). The conclusion of each of these steps is that a certain
+  place in the marked graph is marked. *)
+Print stage_place.
+
+  
+  (*Lemma pipeline_env := *)
+    (* Normal environment: NOT lack lreq ∥ forward rreq rack *)
+    (* Timing constraint: wait for both lack AND rreq before enabling either lreq or rack *)
+    (* Timing constraint: clk should fall BEFORE lreq changes, and clk should fall BEFORE rack changes 
+       NOTE: why is this timing constraint necessary? *)
+Print flop_component.
+
+  Definition left_env_component (l : latch even odd) :=
+    NOT (ack (latch_input l)) (req (latch_input l)).
+  Definition right_env_component (l : latch even odd) :=
+    forward (req (latch_output l)) (ack (latch_output l)).
+
+
+  Record stage_relation_property (σ : state name) (m : marking (stage_MG in_flag out_flag)) :=
+  { (* ENVIRONMENT constraints *)
+    R_left_ack_left_req :
+      σ (ack (latch_input l)) = σ (req (latch_input l)) ->
+      m _ _ left_ack_left_req > 0
+  ; R_right_req_right_ack :
+      σ (req (latch_output l)) = σ (ack (latch_output l)) ->
+      m _ _ right_req_right_ack > 0
+
+    (* TIMING constraints *)
+  ; R_clk_fall_left_req :
+      (* the clock has fallen, and a new left request hasn't happened yet. *)
+      σ (latch_clk l) = Bit0 ->
+      σ (latch_state0 l) <> σ (req (latch_input l)) ->
+      m _ _ clk_fall_left_req > 0
+  ; R_clk_fall_right_ack :
+      σ (latch_clk l) = Bit0 ->
+      σ (latch_state0 l) <> σ (ack (latch_output l)) ->
+      m _ _ clk_fall_right_ack > 0
+
+  (* TIMING constraints *)
+  ; R_right_req_left_req :
+    (* don't think this is correct/enough *)
+      ~ stable (latch_right_req_component l) σ ->
+      m _ _ right_req_left_req > 0
+  ; R_left_ack_right_ack :
+     (* don't think this is correct/enough *)
+      ~ stable (latch_left_ack_component l) σ ->
+      m _ _ left_ack_right_ack > 0
+
+  ; R_clk_rise_left_ack :
+       ~ stable (latch_flop_component l) σ
+    \/ ~ stable (latch_left_ack_component l) σ ->
+      m _ _ clk_rise_left_ack > 0
+  ; R_clk_rise_right_req :
+       ~ stable (latch_flop_component l) σ 
+    \/ ~ stable (latch_right_req_component l) σ ->
+      m _ _ clk_rise_right_req > 0
+
+  ; R_clk_fall :
+       ~ stable (latch_flop_component l) σ
+    \/ (σ (latch_clk l) = Bit1 /\ ~ stable (latch_clk_component l) σ) ->
+      m _ _ clock_fall > 0
+
+  ; R_left_req_clk_rise :
+       (* a request has come in from the left, but clk+ has not yet occurred.  *)
+       stable (latch_flop_component l) σ (* the flop is stable, so state0 is up-to-date *) ->
+       stable (left_env_component l) σ (* a request has come in on the left *) ->
+       (* either: (1) state0 has not yet propogated to rreq; (2) state0 has
+       propogated to rreq but an acknowledgement has not yet come in on rack; or
+       (3) state0 has propogated to rreq, acknowledgment has come in on rack,
+       but the result has not yet propogated through to clk. *)
+       (  ~ stable (latch_right_req_component l) σ
+       \/ (stable (latch_right_req_component l) σ /\ ~ stable (right_env_component l) σ)
+       \/ (stable (latch_right_req_component l) σ /\ stable (right_env_component l) σ
+          /\ ~ stable (latch_clk_component l) σ)) ->
+       m _ _ left_req_clk_rise > 0
+
+  ; R_right_ack_clk_rise : 
+       (* a request has come in from the right, but clk+ has not yet occurred.  *)
+       stable (latch_flop_component l) σ (* the flop is stable, so state0 is up-to-date *) ->
+       stable (right_env_component l) σ (* an acknowledgement has come in on the right *) ->
+       (* either: (1) state0 has not yet propogated to lack; (2) state0 has
+       propogated to lack but a request has not yet come in on lreq; or
+       (3) state0 has propogated to lack, request has come in on lreq,
+       but the result has not yet propogated through to clk. *)
+       (  ~ stable (latch_left_ack_component l) σ
+       \/ (stable (latch_left_ack_component l) σ /\ ~ stable (left_env_component l) σ)
+       \/ (stable (latch_left_ack_component l) σ /\ stable (left_env_component l) σ
+          /\ ~ stable (latch_clk_component l) σ)) ->
+       m _ _ right_ack_clk_rise > 0
+
+  }.
+
+
+
+(*  Context `{mg_scheme : MG_naming_scheme name _ (stage_MG in_flag out_flag)}.*)
+  Existing Instance stage_MG_scheme.
+
+About transition_name.
+About transition_update_value.
+  Definition transition_event (t : token_transition) (σ : state name) : event name value :=
+    let x := @transition_name name _ (stage_MG in_flag out_flag) _ t in
+    let v := @transition_update_value name _ (stage_MG in_flag out_flag) _ t (σ x) in
+    Event x v.
+
+
+About is_enabled.
+  Inductive state_relate_marking : state name -> marking (stage_MG in_flag out_flag) -> Prop :=
+  | R_init : state_relate_marking (σR l) (init_marking (stage_MG in_flag out_flag))
+  | R_step σ σ' t m m' : 
+    state_relate_marking σ m ->
+    latch_stage l ⊢ σ →{Some (transition_event t σ)} Some σ' ->
+    is_enabled _ t m ->
+    m' = fire t _ m ->
+    state_relate_marking σ' m'
+  | R_Eps σ σ' m:
+    state_relate_marking σ m ->
+    latch_stage l ⊢ σ →{None} Some σ' ->
+    state_relate_marking σ' m
+  .
+
+Lemma in_equiv_ensemble : forall (X Y : Ensemble name) (x : name),
+    x ∈ X ->
+    Y == X ->
+    x ∈ Y.
+Admitted.
+
+  Lemma state_relate_marking_equiv : forall σ t σ',
+    relate_trace name (latch_stage l) (stage_MG_SS l in_flag)
+                      (σR l) init_stage_MG_state
+                      σ t σ' ->
+    state_relate_marking σ (state_to_marking σ').
+  Proof.
+    intros σ t σ' Hrelate.
+    induction Hrelate.
+    * replace (state_to_marking init_stage_MG_state)
+        with  (init_marking (stage_MG in_flag out_flag))
+        by    admit.
+      apply R_init.
+    * eapply R_Eps; eauto.
+    * inversion H1.
+    * inversion H2.
+
+        replace e with (transition_event t0 σ1) in *.
+          2:{ subst. unfold transition_event.
+              f_equal. f_equal.
+              eapply relate_trace_domain; [ auto | | eauto | | ].
+              * intros x. admit (* true *).
+              * unfold space_domain.
+                left.
+                destruct t0;
+                try (right; 
+                  eapply in_equiv_ensemble; [ | apply latch_stage_output];
+                  simpl; solve_set);
+                try (left; 
+                  eapply in_equiv_ensemble; [ | apply latch_stage_input];
+                  simpl; solve_set).
+             * unfold space_domain.
+                left.
+                destruct t0;
+                  try (right; eexists; split; [ | reflexivity]; simpl; intro; decompose_set_structure; fail);
+                  try (left; eexists; split; [ | reflexivity]; simpl; solve_set).
+              }
+          subst.
+
+
+      eapply R_step; eauto. 
+      admit (* true *).
+  Admitted.
+
+
+  (** Intuitively, [prop_marked p σ] is a property that holds on a state σ
+  whenever a related marking m satisfies [m(p) > 0]. *)
+  Inductive prop_marked : forall {t1 t2} (p : stage_place t1 t2) (σ : state name), Prop :=
+  .
+
+  Lemma step_implies_prop_marked : forall σ t σ',
+    latch_stage l ⊢ σ →{Some (transition_event t σ)} Some σ' ->
+    forall t0 (p : stage_place t0 t), prop_marked p σ.
+  Admitted.
+
+  (* Helper lemmas for relate_implies_marked below *)
+  Lemma relate_implies_marked_eps : forall σ σ' m,
+    latch_stage l ⊢ σ →{None} Some σ' ->
+    state_relate_marking σ m ->
+    state_relate_marking σ' m.
+  Admitted.
+
+  Lemma incoming_place_not_marked : forall σ σ' t,
+    latch_stage l ⊢ σ →{Some (transition_event t σ)} Some σ' ->
+    forall t0 (p : stage_place t0 t),
+        ~ prop_marked p σ.
+  Admitted.
+
+  Lemma disjoint_place_marked : forall σ σ' t,
+    latch_stage l ⊢ σ →{Some (transition_event t σ)} Some σ' ->
+    forall t1 t2 (p : stage_place t1 t2),
+      t1 <> t ->
+      t2 <> t ->
+      prop_marked p σ' ->
+      prop_marked p σ.
+  Admitted.
+
+
+  Lemma relate_implies_marked : forall σ m,
+    state_relate_marking σ m ->
+    forall {t1 t2} (p : stage_place t1 t2),
+      prop_marked p σ ->
+      m _ _ p > 0.
+  (* by induction on state_relate_marking *)
+  Admitted.
+
+
+  Theorem state_related_enabled : forall σ σ' t m,
+    latch_stage l ⊢ σ →{Some (transition_event t σ)} Some σ' ->
+    state_relate_marking σ m ->
+    is_enabled _ t m.
+  Proof.
+    intros.
+    Print is_enabled.
+    intros t0 p.
+    assert (prop_marked p σ) by (eapply step_implies_prop_marked; eauto).
+    eapply relate_implies_marked; eauto.
+  Qed.
+
+
+(*
+
+  
+
+
+  Notation "σ1 'R{' t '}' σ2" := (relate_trace name (latch_stage l) (stage_MG_SS l in_flag)
+                      (σR l) init_stage_MG_state
+                      σ1 t σ2)
+    (left associativity, at level 92).
+
+      
 
   Lemma left_req_relation_enabled : forall σ1 t σ2,
     σ1 R{t} σ2 ->
@@ -327,6 +573,8 @@ Section SS_to_TokenMG.
     ~ stable latch_clk_component σ1 ->
     is_enabled (stage_MG in_flag out_flag) clk_fall (state_to_marking σ2).
   Admitted.
+
+*)
   
 
 
@@ -336,6 +584,7 @@ Section SS_to_TokenMG.
     S ⊢ σ →{Some (Event x v)} Some σ' ->
     x ∈ visible_domain S.
   Admitted.
+
 
 
   Lemma MG_relate_trace_step_lemma :
@@ -609,7 +858,7 @@ Admitted.
       exists m. exists t'. split; auto.
   Admitted.
 *)
-        
+*)        
 
   End SS_to_TokenMG.
 
